Weidenbach_Book/IsaSAT/Pointer_LLVM.thy
@@ -112,12 +112,12 @@ context
   nofail (f' x) \<Longrightarrow> llvm_htriple (R x xi) (f xi) (\<lambda>r. (\<lambda>s. \<exists>xa xb. (R xa (fst r) \<and>* S xb (snd r) \<and>* \<up>(RETURN (xa, xb) \<le> f' x)) s) \<and>* \<box>)\<close>
 begin
 
-definition ptr_write where
-  \<open>ptr_write a = f' a\<close>
+definition ptr_write0 where
+  \<open>ptr_write0 a = f' a\<close>
 
 
-definition ptr_write_code :: "'a::llvm_rep ptr \<Rightarrow> ('a ptr \<times> 'e) llM" where
-  \<open>ptr_write_code a = doM {
+definition ptr_write_code0 :: "'a::llvm_rep ptr \<Rightarrow> ('a ptr \<times> 'e) llM" where
+  \<open>ptr_write_code0 a = doM {
     b \<leftarrow> ll_load a;
     (c, d) \<leftarrow> f (b);
     ll_store c a;
@@ -126,19 +126,19 @@ definition ptr_write_code :: "'a::llvm_rep ptr \<Rightarrow> ('a ptr \<times> 'e
 
 lemma bpto_ptr_write_code2: "nofail (f' ys) \<Longrightarrow> llvm_htriple
   (pointer_assn R ys p \<and>* \<up>\<^sub>d (P ys))
-  (ptr_write_code p)
-  (\<lambda>r. (\<lambda>s. \<exists>xa xb. (pointer_assn R xa (fst r) \<and>* S xb (snd r) \<and>* \<up>(RETURN (xa, xb) \<le> ptr_write ys)) s) \<and>* \<box>)"
+  (ptr_write_code0 p)
+  (\<lambda>r. (\<lambda>s. \<exists>xa xb. (pointer_assn R xa (fst r) \<and>* S xb (snd r) \<and>* \<up>(RETURN (xa, xb) \<le> ptr_write0 ys)) s) \<and>* \<box>)"
   supply [vcg_rules] = writer_rule
-  unfolding ptr_write_code_def pointer_assn_def assn_comp_def ptr_write_def
+  unfolding ptr_write_code0_def pointer_assn_def assn_comp_def ptr_write0_def
   apply vcg
   done
 
 end
 
-lemma [simp]: \<open>nofail (ptr_write f' x) \<longleftrightarrow> nofail (f' x)\<close>
-  by (auto simp: ptr_write_def)
+lemma [simp]: \<open>nofail (ptr_write0 f' x) \<longleftrightarrow> nofail (f' x)\<close>
+  by (auto simp: ptr_write0_def)
 
-locale ptr_write_loc =
+locale ptr_write_loc0 =
   fixes f ::  "'a::llvm_rep \<Rightarrow> _" and f' and ptr_assn and b_assn and R and P and S
   assumes H: \<open>(f, f') \<in> [P]\<^sub>a (R)\<^sup>d \<rightarrow> R \<times>\<^sub>a S\<close>
   notes [[sepref_register_adhoc f']]
@@ -147,8 +147,8 @@ begin
 
 lemma ptr_write_code_rule:
   assumes \<open>nofail (f' ys)\<close>
-  shows "llvm_htriple (pointer_assn R ys p \<and>* \<up>\<^sub>dP ys) (ptr_write_code f p)
-    (\<lambda>r. (\<lambda>s. \<exists>xa xb. (pointer_assn R xa (fst r) \<and>*  S xb (snd r) \<and>* \<up>(RETURN (xa, xb) \<le> ptr_write f' ys)) s) \<and>* \<box>)"
+  shows "llvm_htriple (pointer_assn R ys p \<and>* \<up>\<^sub>dP ys) (ptr_write_code0 f p)
+    (\<lambda>r. (\<lambda>s. \<exists>xa xb. (pointer_assn R xa (fst r) \<and>*  S xb (snd r) \<and>* \<up>(RETURN (xa, xb) \<le> ptr_write0 f' ys)) s) \<and>* \<box>)"
   (*supply [vcg_rules] = bpto_ptr_write_code2 does not work it looses track of dependencies between variables*)
   apply vcg
   apply (subst POSTCOND_def)
@@ -170,7 +170,7 @@ defer
   apply assumption
   by (simp add: STATE_extract(2) invalid_assn_def pure_true_conv)
 
-lemma ptr_write_code: \<open>(ptr_write_code f, ptr_write f') \<in> [P]\<^sub>a (pointer_assn R)\<^sup>d \<rightarrow> pointer_assn R \<times>\<^sub>a S\<close>
+lemma ptr_write_code: \<open>(ptr_write_code0 f, ptr_write0 f') \<in> [P]\<^sub>a (pointer_assn R)\<^sup>d \<rightarrow> pointer_assn R \<times>\<^sub>a S\<close>
   supply [vcg_rules] = ptr_write_code_rule
   apply sepref_to_hoare
   apply vcg
@@ -178,6 +178,95 @@ lemma ptr_write_code: \<open>(ptr_write_code f, ptr_write f') \<in> [P]\<^sub>a 
 
 end
 
+
+
+context
+  fixes
+    f :: \<open>'a::llvm_rep \<Rightarrow> 'b :: llvm_rep \<Rightarrow> ('a \<times> 'cc) llM\<close> and
+    R :: \<open>'a2 \<Rightarrow> 'a \<Rightarrow> _\<close> and
+    S :: \<open>'b2 \<Rightarrow> 'b \<Rightarrow> _\<close> and
+    T :: \<open>'cc2 \<Rightarrow> 'cc \<Rightarrow> llvm_amemory \<Rightarrow> bool\<close> and
+    P :: \<open>'a2 \<Rightarrow> 'b2 \<Rightarrow> bool\<close> and
+    f' :: \<open>'a2 \<Rightarrow> 'b2 \<Rightarrow> ('a2 \<times> 'cc2) nres\<close> 
+  assumes writer_rule: \<open>P x a \<Longrightarrow>
+  nofail (f' x a) \<Longrightarrow> llvm_htriple (R x xi \<and>* S a b) (f xi b) (\<lambda>r. S a b \<and>* (\<lambda>s. \<exists>xa xb. (R xa (fst r) \<and>* T xb (snd r) \<and>* \<up>(RETURN (xa, xb) \<le> f' x a)) s))\<close>
+begin
+definition ptr_write where
+  \<open>ptr_write a b = f' a b\<close>
+
+
+definition ptr_write_code :: "'a::llvm_rep ptr \<Rightarrow> _ \<Rightarrow> ('a ptr \<times> 'cc) llM" where
+  \<open>ptr_write_code a d = doM {
+    b \<leftarrow> ll_load a;
+    (c, d) \<leftarrow> f (b) d;
+    ll_store c a;
+    Mreturn (a, d)
+  }\<close>
+
+lemma bpto_ptr_write_code: "nofail (f' ys a) \<Longrightarrow> llvm_htriple
+  (pointer_assn R ys p \<and>* S a b \<and>* \<up>\<^sub>d (P ys a))
+  (ptr_write_code p b)
+  (\<lambda>r. (\<lambda>s. \<exists>xa xb. (S a b \<and>* pointer_assn R xa (fst r) \<and>* T xb (snd r) \<and>* \<up>(RETURN (xa, xb) \<le> ptr_write ys a)) s))"
+  supply [vcg_rules] = writer_rule
+  unfolding ptr_write_code_def pointer_assn_def assn_comp_def ptr_write_def
+  apply vcg
+  done
+
+end
+
+lemma [simp]: \<open>nofail (ptr_write0 f' x) \<longleftrightarrow> nofail (f' x)\<close>
+  by (auto simp: ptr_write0_def)
+
+locale ptr_write_loc =
+  fixes
+    f :: \<open>'a::llvm_rep \<Rightarrow> 'b :: llvm_rep \<Rightarrow> ('a \<times> 'cc) llM\<close> and
+    R :: \<open>'a2 \<Rightarrow> 'a \<Rightarrow> _\<close> and
+    S :: \<open>'b2 \<Rightarrow> 'b \<Rightarrow> _\<close> and
+    T :: \<open>'cc2 \<Rightarrow> 'cc \<Rightarrow> llvm_amemory \<Rightarrow> bool\<close> and
+    P :: \<open>'a2 \<Rightarrow> 'b2 \<Rightarrow> bool\<close> and
+    f' :: \<open>'a2 \<Rightarrow> 'b2 \<Rightarrow> ('a2 \<times> 'cc2) nres\<close> 
+  assumes H: \<open>(uncurry f, uncurry f') \<in> [uncurry P]\<^sub>a (R)\<^sup>d *\<^sub>a S\<^sup>k \<rightarrow> R \<times>\<^sub>a T\<close>
+  notes [[sepref_register_adhoc f']]
+  notes [fcomp_norm_unfold] = pointer_assn_def[symmetric]
+begin
+
+lemma ptr_write_code_rule:
+  assumes \<open>nofail (f' ys a)\<close>
+   shows "llvm_htriple (pointer_assn R ys p \<and>* S a b \<and>* \<up>\<^sub>dP ys a) (ptr_write_code f p b)
+    (\<lambda>r.  (\<lambda>s. \<exists>xa xb. (S a b \<and>* pointer_assn R xa (fst r) \<and>*  T xb (snd r) \<and>* \<up>(RETURN (xa, xb) \<le> ptr_write f' ys a)) s))"
+  (*supply [vcg_rules] = bpto_ptr_write_code2 does not work it looses track of dependencies between variables*)
+  apply vcg
+  apply (subst POSTCOND_def)
+  apply (rule bpto_ptr_write_code[simplified, unfolded hn_ctxt_def hn_refine_def htriple_def
+    sep_conj_empty' pure_true_conv sep.add_assoc, rule_format, where P=P])
+defer
+ apply (rule assms)
+ apply (auto simp: pure_def exists_eq_star_conv' assms SOLVE_AUTO_DEFER_def
+     pure_true_conv)[]
+
+  apply (rule wpa_monoI)
+  apply (rule H[to_hnr, simplified, unfolded hn_ctxt_def hn_refine_def htriple_def
+    sep_conj_empty' pure_true_conv sep.add_assoc, rule_format])
+  apply assumption back
+  apply assumption
+  apply assumption
+  apply (auto simp: pure_def exists_eq_star_conv' assms)
+  apply (rule STATE_monoI)
+  apply assumption
+  by (simp add: STATE_extract(2) invalid_assn_def pure_true_conv)
+find_theorems "(_ \<times>\<^sub>a _)(_,_) (_,_)"
+lemma ptr_write_code: \<open>(uncurry (ptr_write_code f), uncurry (ptr_write f')) \<in> [uncurry P]\<^sub>a (pointer_assn R)\<^sup>d *\<^sub>a S\<^sup>k \<rightarrow> pointer_assn R \<times>\<^sub>a T\<close>
+  supply [vcg_rules] = ptr_write_code_rule[unfolded prod_assn_pair_conv[symmetric]]
+thm ptr_write_code_rule[unfolded prod_assn_pair_conv[of \<open>pointer_assn R\<close> T, symmetric]]
+  prod_assn_pair_conv[of \<open>pointer_assn R\<close> T, symmetric]
+  apply sepref_to_hoare
+  unfolding pure_true_conv sep_conj_empty'
+  apply vcg
+  unfolding pure_true_conv sep_conj_empty' 
+  apply vcg
+  done
+
+end
 
 
 context
